v2/perm.v
@@ -1,27 +1,49 @@
 (* Permutations based on Pmap from std++. *)
 
-Require Import PArith.
-From stdpp Require Import base option list numbers pmap.
+From stdpp Require Export base numbers option list pmap.
 
 Global Open Scope positive_scope.
 Global Open Scope list_scope.
 
-Definition perm_lookup_raw (m : Pmap positive) (i : positive) : positive :=
+Definition pmap_f (m : Pmap positive) (i : positive) : positive :=
   default i (m !! i).
 
-Definition perm_compose_raw (m1 m2 : Pmap positive) : Pmap positive :=
-  merge (from_option Some) m2 (perm_lookup_raw m2 <$> m1).
+Definition pmap_swap (i j : positive) : Pmap positive :=
+  {[i:=j; j:=i]}.
+
+Definition pmap_compose (m1 m2 : Pmap positive) : Pmap positive :=
+  merge (from_option Some) m2 (pmap_f m2 <$> m1).
 
 Lemma contra {P Q : Prop} :
   (P -> Q) -> ¬ Q -> ¬ P.
 Proof. auto. Qed.
 
-Lemma perm_compose_raw_inj (m1 m2 : Pmap positive) :
-  Inj eq eq (perm_lookup_raw m1) ->
-  Inj eq eq (perm_lookup_raw m2) ->
-  Inj eq eq (perm_lookup_raw (perm_compose_raw m1 m2)).
+Lemma pmap_empty_inj :
+  Inj eq eq (pmap_f ∅).
 Proof.
-intros H1 H2 x1 x2; repeat unfold perm_lookup_raw, perm_compose_raw in *.
+Admitted.
+
+Lemma pmap_empty_surj :
+  Surj eq (pmap_f ∅).
+Proof.
+Admitted.
+
+Lemma pmap_swap_inj i j :
+  Inj eq eq (pmap_f (pmap_swap i j)).
+Proof.
+Admitted.
+
+Lemma pmap_swap_surj i j :
+  Surj eq (pmap_f (pmap_swap i j)).
+Proof.
+Admitted.
+
+Lemma pmap_compose_inj (m1 m2 : Pmap positive) :
+  Inj eq eq (pmap_f m1) ->
+  Inj eq eq (pmap_f m2) ->
+  Inj eq eq (pmap_f (pmap_compose m1 m2)).
+Proof.
+intros H1 H2 x1 x2; repeat unfold pmap_f, pmap_compose in *.
 rewrite ?lookup_merge, ?lookup_fmap; intros H3.
 destruct (decide (x1 = x2)) as [H4|H4]; [done|exfalso].
 assert (H5 := contra (H1 _ _) H4); cbn in *;
@@ -30,31 +52,60 @@ assert (H6 := contra (H2 _ _) H5); cbn in *;
 repeat destruct (m2 !! _); done.
 Qed.
 
-Lemma perm_compose_raw_surj (m1 m2 : Pmap positive) :
-  Surj eq (perm_lookup_raw m1) ->
-  Surj eq (perm_lookup_raw m2) ->
-  Surj eq (perm_lookup_raw (perm_compose_raw m1 m2)).
+Lemma pmap_compose_surj (m1 m2 : Pmap positive) :
+  Surj eq (pmap_f m1) ->
+  Surj eq (pmap_f m2) ->
+  Surj eq (pmap_f (pmap_compose m1 m2)).
 Proof.
 intros H1 H2 z; destruct (H2 z) as [y Hy], (H1 y) as [x Hx]; exists x.
-clear H1 H2; unfold perm_lookup_raw, perm_compose_raw in *.
+clear H1 H2; unfold pmap_f, pmap_compose in *.
 rewrite lookup_merge, lookup_fmap; simplify_option_eq.
-destruct (m1 !! x) as [y|]; cbn. unfold perm_lookup_raw.
-destruct (m2 !! x), (m2 !! y); done. destruct (m2 !! x); done.
+destruct (m1 !! x) as [y|]; cbn; unfold pmap_f.
+destruct (m2 !! x), (m2 !! y); done.
+destruct (m2 !! x); done.
 Qed.
 
 Inductive perm := Perm {
   perm_car  : Pmap positive;
-  perm_inj  : Inj eq eq (perm_lookup_raw perm_car);
-  perm_surj : Surj eq (perm_lookup_raw perm_car);
+  perm_inj  : Inj eq eq (pmap_f perm_car);
+  perm_surj : Surj eq (pmap_f perm_car);
 }.
+
+Global Instance : FinMapToList positive positive perm :=
+  λ π, map_to_list (perm_car π).
+
+Global Instance perm_lookup : LookupTotal positive positive perm :=
+  λ i π, pmap_f (perm_car π) i.
+
+Global Instance : Empty perm :=
+  Perm _ pmap_empty_inj pmap_empty_surj.
+
+Definition perm_swap (i j : positive) :=
+  Perm _ (pmap_swap_inj i j) (pmap_swap_surj i j).
 
 Definition perm_compose (π τ : perm) :=
   let (π_m, π_inj, π_surj) := π in
   let (τ_m, τ_inj, τ_surj) := τ in
-  Perm (perm_compose_raw π_m τ_m)
-    (perm_compose_raw_inj _ _ π_inj τ_inj)
-    (perm_compose_raw_surj _ _ π_surj τ_surj).
+  Perm (pmap_compose π_m τ_m)
+    (pmap_compose_inj _ _ π_inj τ_inj)
+    (pmap_compose_surj _ _ π_surj τ_surj).
 
-Notation perm_lookup π := (perm_lookup_raw (perm_car π)).
-Notation "π ⋅ i" := (perm_lookup π i) (at level 5, format "π ⋅ i").
-Notation "π ∘ τ" := (perm_compose π τ).
+Notation "⟨ i ; j ⟩" := (perm_swap i j) (format "⟨ i ;  j ⟩").
+Notation "π ⋅ τ" := (perm_compose τ π) (at level 15).
+
+Definition perm_cycle (i : positive) (is : list positive) : perm :=
+  foldl (λ π j, ⟨i; j⟩ ⋅ π) ∅ is.
+
+Notation "⟨ i ; x ; y ; .. ; z ⟩" :=
+  (perm_cycle i (cons x (cons y .. (cons z nil) ..)))
+  (format "⟨ i ;  x ;  y ;  .. ;  z ⟩").
+
+Theorem lookup_compose π τ i :
+  π ⋅ τ !!! i = π !!! (τ !!! i).
+Proof.
+destruct τ as [τ_m ? ?], π as [π_m ? ?]; unfold lookup_total, perm_lookup; cbn.
+unfold pmap_f, pmap_compose; rewrite lookup_merge, lookup_fmap.
+destruct (τ_m !! i) as [i1|]; cbn; unfold pmap_f.
+destruct (π_m !! i) as [i0|], (π_m !! i1); done.
+destruct (π_m !! i) as [i0|]; done.
+Qed.
